Add syntax for sig

syntax.sig
@@ -11,3 +11,6 @@ tAbsurd : tm -> tm
 tEq : T -> tm -> tm -> tm -> tm
 tJ : (tm -> tm -> tm) -> tm -> tm -> tm
 tRefl : tm
+tSig : T -> tm -> (tm -> tm) -> tm
+tPack : T -> tm -> tm -> tm
+tLet : T -> T -> tm -> (tm -> tm -> tm) -> tm
